theories/encryption/PKE.ec
@@ -18,340 +18,228 @@ module type Scheme = {
   fun kg() : pkey * skey 
   fun enc(pk:pkey, m:plaintext)  : ciphertext 
   fun dec(sk:skey, c:ciphertext) : plaintext option  
-  fun leaks(
-   
 }.
-theory CPA.
 
-  type 
- 
+module Correctness (S:Scheme) = {
+  fun main(m:plaintext) : bool = {
+    var pk : pkey;
+    var sk : skey;
+    var c  : ciphertext;
+    var m' : plaintext option;
 
-  module type Adversary = {
-    fun choose(pk:pkey)     : plaintext * plaintext 
-    fun guess(c:ciphertext) : bool                  
-  }.
-
-  
-clone import Indist
-
-module CPA
-type input.
-
-clone import Hybrid as H 
-  with type input <- input * input,
-       type outputA <- bool.
-
-module type Orcl = {
-  fun leaks (il:inleaks) : outleaks  
-  fun orcl (m:input) : output
+    (pk, sk) = S.kg();
+    c        = S.enc(pk, m);
+    m'       = S.dec(sk, c); 
+    return (m' = Some m);
+  }
 }.
 
 module type LR = {
-  fun orcl (m0 m1:input) : output
+  fun orcl (m0 m1:plaintext) : ciphertext
 }.
 
-module OrclL (O:Orcl) = {
+module type AdvCPA(LR:LR) = {
+  fun main(pk:pkey) : bool
+}.
 
-  fun orcl (m0 m1:input) : output = {
-    var r : output;
-    r = O.orcl(m0);
-    C.incr();
+module K = { 
+  var c  : int
+  var pk : pkey
+  var sk : skey
+  var b  : bool
+}.
+ 
+module L (S:Scheme) = {
+
+  fun orcl (m0 m1:plaintext) : ciphertext = {
+    var r : ciphertext;
+    r = S.enc(K.pk,m0);
+    K.c = K.c + 1;
     return r;
   }
 }.
 
-module OrclR (O:Orcl) = {
-  fun init () : unit = { C.init(); }
+module R (S:Scheme) = {
 
-  fun orcl (m0 m1:input) : output = {
-    var r : output;
-    C.incr();
-    r = O.orcl(m1);
+  fun orcl (m0 m1:plaintext) : ciphertext = {
+    var r : ciphertext;
+    r = S.enc(K.pk,m1);
+    K.c = K.c + 1;
     return r;
   }
 }.
 
-module Orclb (O:Orcl) = {
+module LRb (S:Scheme) = {
 
-  var b:bool
-  fun orcl (m0 m1:input) : output = {
-    var r : output;
-    C.incr();
-    r = O.orcl(b?m0:m1);
+  fun orcl (m0 m1:plaintext) : ciphertext = {
+    var r : ciphertext;
+    r = S.enc(K.pk,K.b?m0:m1);
+    K.c = K.c + 1;
     return r;
   }
 }.
 
-module type Adv (O:Orcl, LR:LR) = { fun main():bool { O.leaks O.orcl LR.orcl }}.
-
-module INDL (O:Orcl, A:Adv) = {
-  module A = A(O,OrclL(O))
-  fun main():bool = {
-    var b' : bool;
-    C.init();
-    b' = A.main();
-    return b';
-  }
-}.
-
-module INDR (O:Orcl, A:Adv) = {
-  module A = A(O,OrclR(O))
-  fun main():bool = {
-    var b' : bool;
-    C.init();
-    b' = A.main();
-    return b';
-  }
-}.
-
-module INDb(O:Orcl,A:Adv) = {
-  module A = A(O,Orclb(O))
-  fun main():bool = {
-    var b' : bool;
-    C.init();
-    Orclb.b = ${0,1};
-    b' = A.main();
-    return Orclb.b = b';
-  }
-}.
-
-(* We prove the equivalence between the two usual definitions *)
-(* i.e (INDb - 1/2) = (INDL - INDR)/2 *)
-
-section.
-  declare module O:Orcl {C, Orclb}.
-  declare module A:Adv  {C, O, Orclb}.
-
-  local module WA = {
-    module A=A(O,Orclb(O))  
-    fun work(x:bool) : bool = {
-      var b' : bool;
-      C.init();
-      Orclb.b = x;
-      b' = A.main();
-      return b';
-    }
-  }.
-
-  lemma INDb_INDLR &m (p:glob A -> glob O -> int -> bool):
-     Pr[INDb(O,A).main() @ &m : res /\ p (glob A) (glob O) C.c] -
-       Pr[INDR(O,A).main() @ &m : p (glob A) (glob O) C.c]/2%r =
-     (Pr[INDL(O,A).main() @ &m : res /\ p (glob A) (glob O) C.c] -
-      Pr[INDR(O,A).main() @ &m : res /\ p (glob A) (glob O) C.c])/2%r.
-  proof strict.
-   cut := Sample_bool WA &m 
-     (lambda (g:glob WA), let (b,c,go,ga) = g in p ga go c) => /= H.
-   cut -> : Pr[INDb(O, A).main() @ &m : res /\ p (glob A) (glob O) C.c] =
-    Pr[MB.M.Rand(WA).main() @ &m : fst res = snd res /\ p (glob A) (glob O) C.c].
-     equiv_deno (_: ={glob A,glob O} ==> ={glob A,glob O, C.c} /\
-                   res{1} = (fst res = snd res){2}) => //;fun.
-     inline C.init WA.work;simplify fst snd. 
-     by swap{1} 2 -1; eqobs_in; fun (={Orclb.b, C.c}).
-   cut He: equiv [INDR(O, A).main ~ WA.work: x{2}=false /\ 
-                   ={glob A,glob O} ==> ={res,glob A,glob O, C.c}].
-    fun. 
-    call (_: ={glob O, C.c} /\ Orclb.b{2} = false).
-      by fun (={C.c} /\ Orclb.b{2} = false).      
-      by fun (={C.c} /\ Orclb.b{2} = false). 
-      by fun;inline C.incr;wp;call(_:true);wp;skip;progress.
-    inline C.init;by wp.
-   cut -> : Pr[INDR(O, A).main() @ &m : p (glob A) (glob O) C.c] =
-            Pr[WA.work(false) @ &m : p (glob A) (glob O) C.c].
-     by equiv_deno He.
-   cut -> : Pr[INDR(O, A).main() @ &m : res /\ p (glob A) (glob O) C.c] = 
-            Pr[WA.work(false) @ &m : res /\ p (glob A) (glob O) C.c].
-     by equiv_deno He.
-   (cut -> : Pr[INDL(O, A).main() @ &m : res /\ p (glob A) (glob O) C.c] = 
-            Pr[WA.work(true) @ &m : res /\ p (glob A) (glob O) C.c]) => //.
-   equiv_deno 
-      (_: x{2}=true /\ ={glob A,glob O} ==> ={res,glob A,glob O, C.c}) => //.
-   fun; call (_: ={glob O, C.c} /\ Orclb.b{2} = true).
-     by fun (={C.c} /\ Orclb.b{2} = true).      
-     by fun (={C.c} /\ Orclb.b{2} = true). 
-     by fun;inline C.incr;wp;call(_:true);wp;skip;progress.
-   inline C.init;by wp.
- qed.
-
-end section.
-
-(* We prove that IND-n is equivalent to IND-1 *)
-
-module Orcl2(O:Orcl) = {
-  fun leaks (il:inleaks) : outleaks = {
-    var r : outleaks;
-    r = O.leaks(il);
-    return r;
-  }
-
-  fun orcl1 (m:input * input) : output = {
-    var r : output;
-    r = O.orcl(fst m);
-    return r;
-  }
-
-  fun orcl2 (m:input * input) : output = {
-    var r : output;
-    r = O.orcl(snd m);
-    return r;
-  }  
-}.
-
-module LRB2 (O:Orcl,LR:LR) = {
-  fun orcl(m0 m1:input):output = {
-    var r : output;
-    if (LRB.l0 < LRB.l) r = O.orcl(m0);
-    else { 
-      if (LRB.l0 = LRB.l) r = LR.orcl(m0,m1);
-      else r = O.orcl(m1);
-    }
-    LRB.l = LRB.l + 1;
-    return r;
-  }    
-}.
-
-module B(A:Adv, O:Orcl, LR:LR) = {
-  module A = A(O,LRB2(O,LR))
+module CPAL (S:Scheme,A:AdvCPA) = {
+  module A = A(L(S))
   fun main():bool = {
     var b':bool;
-    LRB.l0 = $[0..q-1];
-    LRB.l  = 0;
-    b' = A.main();
+    K.c = 0;
+    (K.pk,K.sk) = S.kg();
+    b' = A.main(K.pk);
+    return b';
+  }
+}.
+
+module CPAR (S:Scheme,A:AdvCPA) = {
+  module A = A(R(S))
+  fun main():bool = {
+    var b':bool;
+    K.c = 0;
+    (K.pk,K.sk) = S.kg();
+    b' = A.main(K.pk);
+    return b';
+  }
+}.
+
+module CPA (S:Scheme,A:AdvCPA) = {
+  module A = A(LRb(S))
+  fun main():bool = {
+    var b':bool;
+    K.c = 0;
+    K.b = ${0,1};
+    (K.pk,K.sk) = S.kg();
+    b' = A.main(K.pk);
+    return b';
+  }
+}.
+
+clone import Indist as Ind with
+  type input <- plaintext,
+  type H.output <- ciphertext,
+  type H.inleaks <- unit,
+  type H.outleaks <- pkey.
+
+module ToOrcl (S:Scheme) = {
+  fun leaks (il:unit) : pkey = {
+    (K.pk, K.sk) = S.kg();
+    return K.pk;
+  }
+  fun orcl (m:plaintext) : ciphertext = {
+    var c : ciphertext;
+    c = S.enc(K.pk, m);
+    return c;
+  }
+}.
+
+module ToAdv(A:AdvCPA, O:Orcl,LR:LR) = {
+  module A = A(LR)
+  fun main() : bool = {
+    var pk:pkey;
+    var b':bool;
+    pk = O.leaks(());
+    b' =A.main(pk);
+    return b';
+  }
+}.
+
+module B (S:Scheme, A:AdvCPA, LR:LR) = {
+  module A = A(LRB2(ToOrcl(S),LR))
+  fun main(pk:pkey) : bool = {
+    var b':bool;
+    H.LRB.l0 = $[0..H.q-1];
+    H.LRB.l  = 0;
+    b' = A.main(pk);
     return b';
   }
 }.
 
 section.
 
-  declare module O:Orcl {C, LRB}.
-  declare module A:Adv  {C, O, LRB}.
+  declare module S:Scheme {K, H.C, H.LRB}. 
+    (* Normaly I would like to locally 
+       clone Indist in the section, in that case
+       restrictions at least on H.c are not needed.
+       But LRB and B are used so we need to do it 
+     *) 
 
-  local module A' (Ob:Orclb, LR:H.Orcl) = {
-    module O = {
-      fun leaks(il:inleaks) : outleaks = {
-        var r : outleaks;
-        r = Ob.leaks(il);
-        return r;
-      }
-      fun orcl(m:input) : output = {
-        var r:output;
-        r = Ob.orcl1((m,m));
-        return r;
-      }
-    }
-    module LR' = {
-      fun orcl (m0 m1:input) : output = {
-        var r : output;
-        r = LR.orcl((m0,m1));
-        return r;
-      }
-    }
-    module A = A(O,LR')
-    fun main():bool = {
-      var b':bool;
-      b' = A.main();
-      return b';
-    }
-  }.
+  declare module A:AdvCPA {K,H.C,H.LRB,S}.
 
-  axiom losslessL: islossless O.leaks.
-  axiom losslessO: islossless O.orcl. 
-  axiom losslessA (O <: Orcl{A}) (LR <: LR{A}):
-    islossless LR.orcl => 
-    islossless O.leaks => islossless O.orcl =>
-    islossless A(O, LR).main.
-  axiom q_pos : 0 < q.     
-         
-  lemma IND1_INDn &m (p:glob A -> glob O -> int -> bool):
-     Pr[INDL(O,B(A)).main() @ &m : res /\ p (glob A) (glob O) LRB.l /\
-                                    LRB.l <= q /\ C.c <= 1] - 
-       Pr[INDR(O,B(A)).main() @ &m : res /\ p (glob A) (glob O) LRB.l /\
-                                    LRB.l <= q /\ C.c <= 1]  =
-     1%r/q%r * (
-       Pr[INDL(O,A).main() @ &m : res /\ p (glob A) (glob O) C.c /\
-                                  C.c <= q] - 
-         Pr[INDR(O,A).main() @ &m :  res /\ p (glob A) (glob O) C.c /\
-                                  C.c <= q]).
+  axiom Lkg  : islossless S.kg.
+  axiom Lenc : islossless S.enc. 
+  axiom La   : forall (LR<:LR{A}), islossless LR.orcl => islossless A(LR).main.
+
+  equiv CPAL_INDL (A0<:AdvCPA {K,H.C,S}) : 
+        CPAL(S,A0).main ~ INDL(ToOrcl(S),ToAdv(A0)).main : ={glob A0, glob S} ==>
+           ={res,glob A0, glob S, K.pk} /\ K.c{1} = H.C.c{2}.
   proof.
-    cut := Hybrid (Orcl2(O)) A' _ _ _ _ _ &m (lambda ga go c b, b /\ p ga go c).
-      by fun;call losslessL.
-      by fun;call losslessO.
-      by fun;call losslessO.
-      intros Ob LR Hlr Hl Ho1 Ho2;fun.
-      by call (losslessA (<:A'(Ob,LR).O) (<:A'(Ob,LR).LR') _ _ _) => //;fun;
-        [call Hlr | call Hl | call Ho1].
-      apply q_pos.
-    zeta beta => H.
-    cut -> : Pr[INDL(O, B(A)).main() @ &m :
-                 res /\ p (glob A) (glob O) LRB.l /\ LRB.l <= q /\ C.c <= 1] =
-             Pr[Ln(Orcl2(O), H.B(A')).main() @ &m :
-                 ((res /\ p (glob A) (glob O) LRB.l) /\ LRB.l <= q) /\ C.c <= 1].
-      equiv_deno (_: ={glob A,glob O} ==>
-                     ={res,glob A,glob O,glob LRB, C.c}) => //;fun.
-      call (_: ={glob A,glob O, C.c} ==> ={glob A,glob O,glob LRB,C.c,res}).
-        fun;inline H.B(A', Orcl2(O), Orclc(L(Orcl2(O)))).A.main;wp.
-        call (_: ={glob O, C.c, glob LRB}).
-          fun *. inline A'(Orcl2(O), LRB(Orcl2(O), Orclc(L(Orcl2(O))))).O.leaks Orcl2(O).leaks;wp.
-          by call (_:true);wp.
-          fun *. inline A'(Orcl2(O), LRB(Orcl2(O), Orclc(L(Orcl2(O))))).O.orcl Orcl2(O).orcl1;wp.
-          by call (_:true);wp.
-          fun. inline LRB(Orcl2(O), Orclc(L(Orcl2(O)))).orcl Orcl2(O).orcl1 Orcl2(O).orcl2;wp.
-          sp;if => //;first by wp;call (_:true);wp.
-          if => //;last by wp;call (_:true);wp.
-          inline OrclL(O).orcl Orclc(L(Orcl2(O))).orcl L(Orcl2(O)).orcl Orcl2(O).orcl1 C.incr.
-          by wp;call (_: true);wp.
-        by wp;rnd.
-      by call (_:true ==> ={C.c});first by fun;wp.
-    cut -> : Pr[INDR(O, B(A)).main() @ &m :
-                 res /\ p (glob A) (glob O) LRB.l /\ LRB.l <= q /\ C.c <= 1] =
-             Pr[Rn(Orcl2(O), H.B(A')).main() @ &m :
-                 ((res /\ p (glob A) (glob O) LRB.l) /\ LRB.l <= q) /\ C.c <= 1].
-      equiv_deno (_: ={glob A,glob O} ==>
-                     ={res,glob A,glob O,glob LRB, C.c}) => //;fun.
-      call (_: ={glob A,glob O, C.c} ==> ={glob A,glob O,glob LRB,C.c,res}).
-        fun;inline H.B(A', Orcl2(O), Orclc(R(Orcl2(O)))).A.main;wp.
-        call (_: ={glob O, C.c, glob LRB}).
-          fun *. inline A'(Orcl2(O), LRB(Orcl2(O), Orclc(R(Orcl2(O))))).O.leaks Orcl2(O).leaks;wp.
-          by call (_:true);wp.
-          fun *. inline A'(Orcl2(O), LRB(Orcl2(O), Orclc(R(Orcl2(O))))).O.orcl Orcl2(O).orcl1;wp.
-          by call (_:true);wp.
-          fun. inline LRB(Orcl2(O), Orclc(R(Orcl2(O)))).orcl Orcl2(O).orcl1 Orcl2(O).orcl2;wp.
-          sp;if => //;first by wp;call (_:true);wp.
-          if => //;last by wp;call (_:true);wp.
-          inline OrclR(O).orcl Orclc(R(Orcl2(O))).orcl R(Orcl2(O)).orcl Orcl2(O).orcl2 C.incr.
-          by wp;call (_: true);wp.
-        by wp;rnd.
-      by call (_:true ==> ={C.c});first by fun;wp.
-   (* BUG : rewrite H.  *)
-   cut -> : Pr[INDL(O, A).main() @ &m : res /\ p (glob A) (glob O) C.c /\ C.c <= q] =
-            Pr[Ln(Orcl2(O), A').main() @ &m : (res /\ p (glob A) (glob O) C.c) /\ C.c <= q].
-     equiv_deno (_: ={glob A,glob O} ==>
-                    ={res,glob A,glob O, C.c}) => //;fun.
-      call (_: ={glob A,glob O, C.c} ==> ={glob A,glob O,C.c,res}).
-        fun *. inline A'(Orcl2(O), Orclc(L(Orcl2(O)))).main;eqobs_in.
-        call (_: ={glob O, C.c}) => //.
-          fun *. inline A'(Orcl2(O), Orclc(L(Orcl2(O)))).O.leaks Orcl2(O).leaks;wp.
-          by call (_:true);wp.
-          fun *. inline A'(Orcl2(O), Orclc(L(Orcl2(O)))).O.orcl Orcl2(O).orcl1;wp.
-          by call (_:true);wp.
-          fun;inline Orclc(L(Orcl2(O))).orcl L(Orcl2(O)).orcl Orcl2(O).orcl1 C.incr.
-        by wp;call(_:true);wp.
-      by call (_:true ==> ={C.c});first by fun;wp.
-   cut -> : Pr[INDR(O, A).main() @ &m : res /\ p (glob A) (glob O) C.c /\ C.c <= q] =
-            Pr[Rn(Orcl2(O), A').main() @ &m : (res /\ p (glob A) (glob O) C.c) /\ C.c <= q].
-     equiv_deno (_: ={glob A,glob O} ==>
-                    ={res,glob A,glob O, C.c}) => //;fun.
-      call (_: ={glob A,glob O, C.c} ==> ={glob A,glob O,C.c,res}).
-        fun *. inline A'(Orcl2(O), Orclc(R(Orcl2(O)))).main;eqobs_in.
-        call (_: ={glob O, C.c}) => //.
-          fun *. inline A'(Orcl2(O), Orclc(R(Orcl2(O)))).O.leaks Orcl2(O).leaks;wp.
-          by call (_:true);wp.
-          fun *. inline A'(Orcl2(O), Orclc(R(Orcl2(O)))).O.orcl Orcl2(O).orcl1;wp.
-          by call (_:true);wp.
-          fun;inline Orclc(R(Orcl2(O))).orcl R(Orcl2(O)).orcl Orcl2(O).orcl2 C.incr.
-        by wp;call(_:true);wp.
-      by call (_:true ==> ={C.c});first by fun;wp.
-    apply H.
+    fun. 
+    inline INDL(ToOrcl(S), ToAdv(A0)).A.main H.C.init  ToOrcl(S).leaks.
+    wp;call (_: ={glob S, K.pk} /\ K.c{1} = H.C.c{2}).
+      by fun;inline ToOrcl(S).orcl H.C.incr;wp;call (_:true);wp.
+    by wp;call (_:true);wp.
   qed.
 
-end section.
+  equiv CPAR_INDR (A0<:AdvCPA {K,H.C,S}) : 
+        CPAR(S,A0).main ~ INDR(ToOrcl(S),ToAdv(A0)).main : ={glob A0, glob S} ==>
+           ={res,glob A0, glob S, K.pk} /\ K.c{1} = H.C.c{2}.
+  proof.
+    fun. 
+    inline INDR(ToOrcl(S), ToAdv(A0)).A.main H.C.init  ToOrcl(S).leaks.
+    wp;call (_: ={glob S, K.pk} /\ K.c{1} = H.C.c{2}).
+      by fun;inline ToOrcl(S).orcl H.C.incr;wp;call (_:true);wp.
+    by wp;call (_:true);wp.
+  qed.
 
+
+  lemma CPA1_CPAn &m : 0 < H.q => 
+    Pr[CPAL(S,B(S,A)).main() @ &m : res /\ H.LRB.l <= H.q /\ K.c <= 1] - 
+    Pr[CPAR(S,B(S,A)).main() @ &m : res /\ H.LRB.l <= H.q /\ K.c <= 1] =
+    1%r/H.q%r * (Pr[CPAL(S,A).main() @ &m : res /\ K.c <= H.q] -
+                 Pr[CPAR(S,A).main() @ &m : res /\ K.c <= H.q]).
+  proof.
+    intros Hq.
+    cut -> : Pr[CPAL(S, A).main() @ &m : res /\ K.c <= H.q] =
+             Pr[INDL(ToOrcl(S),ToAdv(A)).main() @ &m : res /\ H.C.c <= H.q].
+      by equiv_deno (CPAL_INDL A).
+    cut -> : Pr[CPAR(S, A).main() @ &m : res /\ K.c <= H.q] =
+             Pr[INDR(ToOrcl(S),ToAdv(A)).main() @ &m : res /\ H.C.c <= H.q].          
+      by equiv_deno (CPAR_INDR A).
+    cut := IND1_INDn (ToOrcl(S)) (ToAdv(A)) _ _ _ _ &m (lambda ga go c, true) => //=.
+      by fun;call Lkg.
+      by fun;call Lenc.    
+      intros O LR Llr Ll Lo;fun;call (La LR _) => //.
+      by call Ll.
+    intros <-;congr.
+      equiv_deno (_: ={glob S,glob A} ==> ={res,glob H.LRB} /\ K.c{1} = H.C.c{2}) => //.
+      fun.
+      inline INDR(ToOrcl(S), Ind.B(ToAdv(A))).A.main H.C.init CPAR(S, B(S,A)).A.main
+        Ind.B(ToAdv(A), ToOrcl(S), OrclR(ToOrcl(S))).A.main.
+      wp.
+      call (_: ={glob S,glob H.LRB, K.pk} /\ K.c{1} = H.C.c{2}).
+        fun;wp.
+        if => //.
+          by call (_: ={glob S, K.pk});first eqobs_in.
+        if => //.
+          call (_: ={glob S, K.pk} /\ K.c{1} = H.C.c{2}) => //.
+          by inline ToOrcl(S).orcl H.C.incr;wp;call (_: true);wp.
+        by call (_: ={glob S, K.pk});first eqobs_in.
+      swap{1} [4..5] -2;inline ToOrcl(S).leaks;wp.
+      by call (_:true);wp;rnd;wp.
+    equiv_deno (_: ={glob S,glob A} ==> ={res,glob H.LRB} /\ K.c{1} = H.C.c{2}) => //.
+    fun.
+    inline INDL(ToOrcl(S), Ind.B(ToAdv(A))).A.main H.C.init CPAL(S, B(S,A)).A.main
+      Ind.B(ToAdv(A), ToOrcl(S), OrclL(ToOrcl(S))).A.main.
+    wp.
+    call (_: ={glob S,glob H.LRB, K.pk} /\ K.c{1} = H.C.c{2}).
+      fun;wp.
+      if => //.
+        by call (_: ={glob S, K.pk});first eqobs_in.
+      if => //.
+        call (_: ={glob S, K.pk} /\ K.c{1} = H.C.c{2}) => //.
+        by inline ToOrcl(S).orcl H.C.incr;wp;call (_: true);wp.
+      by call (_: ={glob S, K.pk});first eqobs_in.
+    swap{1} [4..5] -2;inline ToOrcl(S).leaks;wp.
+    by call (_:true);wp;rnd;wp.
+  qed.
+
+end section. 
